Description of the tile puzzle.

theories/tiles.v
@@ -1,7 +1,23 @@
 
-(* TODO: Explain the problem *)
+From Lib Require Import common.
+Open Scope nat_scope.
 
-Record game_state := {
+(** This problem was given to me by Rao Xiaojia.
+  It is about a two-player game in which players remove tiles in a two-dimensional grid. **)
+
+(** Let us consider a finite set of tiles, as follows:
+[[
+  O X X X X X X X X X X X X X X X X X X X X X
+  X X X X X X X X X X X X X X X X X X X X X X
+  X X X X X X X X X X X X X X X X X X X X X X
+  X X X X X X X X X X X X X X X X X X X X X X
+  X X X X X X X X X X X X X X X X X X X X X X
+]]
+
+  Each [X] represents a tile.
+  The origin [O] is special: it can never be removed. **)
+
+Record board := {
     length : nat * nat ;
     state : nat -> nat -> bool ;
     state_out_x : forall x y, x >= fst length -> state x y = false ;
@@ -9,8 +25,8 @@ Record game_state := {
     state_origin : state 0 0 = true
   }.
 
-(** With this definition, we know that there is at least one tile. **)
-Lemma game_state_length_gt_0 : forall st : game_state,
+(** The board is never void: there is at least the origin tile. **)
+Lemma board_length_gt_0 : forall st : board,
   fst (length st) <> 0 /\ snd (length st) <> 0.
 Proof.
   intro st. pose (E := state_origin st).
@@ -22,4 +38,164 @@ Proof.
     + now inversion E.
     + now rewrite E0; auto.
 Qed.
+
+(** The initial board is simply filled with tiles. **)
+Program Definition initial x y (Ix : x > 0) (Iy : y > 0) := {|
+    length := (x, y) ;
+    state := fun x' y' => (x' <? x) && (y' <? y)
+  |}.
+Next Obligation.
+Proof.
+  do 2 erewrite Nat.ltb_antisym. now erewrite leb_correct.
+Qed.
+Next Obligation.
+Proof.
+  do 2 erewrite Nat.ltb_antisym. erewrite andb_comm. now erewrite leb_correct.
+Qed.
+Next Obligation.
+Proof.
+  do 2 erewrite Nat.ltb_antisym. now repeat erewrite leb_correct_conv.
+Qed.
+
+(** The rules of the game are simple: at each turn, the current player chooses
+  a [X] tile.  Then every tile below or right of the chosen tile (including the
+  current tile itself) is removed from the game.
+
+  For instance, the first player can remove the following [-] tiles:
+[[
+  O X X X X X X X X X X X X X X X X X X X X X
+  X X X X X X X X X X X X X X X X X X X X X X
+  X X X X X X X X X X X X X X X X - - - - - -
+  X X X X X X X X X X X X X X X X - - - - - -
+  X X X X X X X X X X X X X X X X - - - - - -
+]]
+
+  Then the second player can continue by removing the following tiles:
+[[
+  O X X X X X X X X X X X X X X X X X X X X X
+  X X X X X X X X X X X X X X X X X X X X X X
+  X X X X X X X X X X X X X X X X            
+  X X X X X X X X - - - - - - - -            
+  X X X X X X X X - - - - - - - -            
+]]
+
+  The first player who can no longer play looses.
+**)
+
+Record turn (st st' : board) x y : Prop := {
+    turn_valid : state st x y = true ;
+    turn_update : forall x' y',
+      state st' x' y' =
+        if (x' <? x) || (y' <? y) then
+          state st x' y'
+        else false
+  }.
+
+(** Reconstruct the board from a position [(x, y)]. **)
+Program Definition make_turn st x y (valid : state st x y = true) (not_origin : x <> 0 \/ y <> 0) := {|
+    length := length st ;
+    state x' y' :=
+      if (x' <? x) || (y' <? y) then
+        state st x' y'
+      else false
+  |}.
+Next Obligation.
+Proof.
+  destruct orb; auto. now apply state_out_x.
+Qed.
+Next Obligation.
+Proof.
+  destruct orb; auto. now apply state_out_y.
+Qed.
+Next Obligation.
+Proof.
+  rewrite state_origin. destruct orb eqn: E; auto.
+  destruct (orb_false_elim _ _ E) as [E1 E2].
+  apply Nat.ltb_ge in E1. apply Nat.ltb_ge in E2.
+  apply le_n_0_eq in E1. apply le_n_0_eq in E2. subst.
+  now destruct not_origin as [D|D].
+Qed.
+
+Lemma make_turn_correct : forall st x y valid not_origin,
+  turn st (make_turn st x y valid not_origin) x y.
+Proof.
+  intros st x y valid not_origin. now constructor.
+Qed.
+
+(** If the current player can’t play, than only the origin is left on the board. **)
+Lemma no_turn_only_origin : forall st,
+  (forall st' x y, ~ turn st st' x y) -> forall x y,
+  state st x y = true <-> x = 0 /\ y = 0.
+Proof.
+  intros st N x y. destruct ((x =? 0) && (y =? 0)) eqn: E.
+  - apply andb_true_iff in E. destruct E as [E1 E2].
+    apply beq_nat_true in E1. apply beq_nat_true in E2.
+    subst. split; auto.
+    intro. apply state_origin.
+  - apply andb_false_iff in E.
+    assert (not_origin : x <> 0 \/ y <> 0).
+    { now destruct E as [E|E]; apply beq_nat_false in E; [ left | right ]. }
+    destruct E as [E|E]; apply beq_nat_false in E;
+      (split; [ intros E'; exfalso; eapply N; apply (make_turn_correct _ _ _ E' not_origin)
+              | now intros [? ?]; subst ]).
+Qed.
+
+(** The puzzle is then the following: for which value of [x] and [y] is there a winning
+  strategy for the first player starting from [initial x y _ _]? **)
+
+(** If [x = y = 1], then only the origin is there and the first player immediately looses. **)
+
+Lemma x_y_1 : forall st x y,
+  ~ turn (initial 1 1 ltac:(apply gt_Sn_O) ltac:(apply gt_Sn_O)) st x y.
+Proof.
+  intros st x y turn.
+  assert (Exy : x = 0 /\ y = 0).
+  {
+    pose (E := turn_valid _ _ _ _ turn).
+    simpl in E. apply andb_true_iff in E. destruct E as [E1 E2].
+    apply Nat.ltb_lt in E1. apply Nat.ltb_lt in E2.
+    apply Nat.lt_1_r in E1. now apply Nat.lt_1_r in E2.
+  }
+  destruct Exy as [? ?]. subst.
+  pose (E := turn_update _ _ _ _ turn 0 0).
+  simpl in E. now rewrite state_origin in E.
+Qed.
+
+(** My first approach was to explore strategies.
+  For instance, here is a nice winning strategy if given a square:
+[[
+  O X X X X
+  X X X X X
+  X X X X X
+  X X X X X
+  X X X X X
+]]
+  The first move consists in taking the tile [(1, 1)]:
+[[
+  O X X X X
+  X - - - -
+  X - - - -
+  X - - - -
+  X - - - -
+]]
+  Then, the idea is to mimick what the second players does on the other branch.
+  For instance, if the second player does:
+[[
+  O X X - -
+  X        
+  X        
+  X        
+  X        
+]]
+  Just make the symmetrical move:
+[[
+  O X X    
+  X        
+  X        
+  -        
+  -        
+]]
+  This will continue until the second player will no longer be able to play. **)
+
+(* TODO *)
 
