lib/common.v
@@ -1,6 +1,7 @@
 (** Some very basic definitions, already present in quite a lot of libraries. **)
 
 From Coq Require Export Bool.Bool.
+From Coq Require Export PeanoNat  Arith.Arith Arith.Compare_dec.
 
 Definition decidable P := { P } + { ~ P }.
 
